thys/examples/sorting/Sorting_Final_insertion_Sort.thy
@@ -601,7 +601,7 @@ context sort_impl_context begin
   sepref_def final_insertion_sort_impl is "uncurry2 (PR_CONST final_insertion_sort3)" 
     :: "(array_assn elem_assn)\<^sup>d *\<^sub>a size_assn\<^sup>k *\<^sub>a size_assn\<^sup>k \<rightarrow>\<^sub>a array_assn elem_assn"
     unfolding final_insertion_sort3_def PR_CONST_def
-    apply (annot_snat_const "TYPE(size_t)")
+    apply (annot_snat_const "TYPE('size_t)")
     by sepref
  
 
